---
title: Inverse Functions
date: 2021-11-24
---
## Inverse Functions

When writing an inverse function, you write the function in the form  $y = ...$ and interchange the xs and ys. And change the form of the equation such that y is alone in one side of the equation. This does not always apply for polynomials. In the case of second-order polynomials for example, you use the formulae $\frac{-b \pm \sqrt{b^2-4ac}}{2a}$ . An  example of taking the inverse of the function $f(x) = x^2 - 4x + 7$ for $x \ge 2$.

$$y = x^2 - 4x + 7$$
$$x = y^2 - 4y + 7$$
$$0 = y^2 - 4y + 7 - x$$ 
$$a=1, b=-4, c=7-x$$
$$y = \frac{4 \pm \sqrt{16 - 4(7-x)}}{2}$$
$$y = \frac{4 \pm 2\sqrt{4 - 7+x}}{2}$$
$$y = 2 \pm \sqrt{x-3}$$
Two possible options:
$$y = 2 + \sqrt{x-3}$$
$$y = 2 - \sqrt{x-3}$$
Since when we take the inverse functions, we switch the domain and the range, we pick the function with the range $y \ge 2$, so the first one. Therefore:

$$f^{-1}(x) = 2 + \sqrt{x-3}$$